WIP

code/ecdsap256/dist/Hacl_P256.c
@@ -400,6 +400,11 @@ static inline void p256_sub(uint64_t *arg1, uint64_t *arg2, uint64_t *out)
   uint64_t c = cc30;
 }
 
+static void p256_neg(uint64_t *arg1)
+{
+  
+}
+
 static inline void montgomery_multiplication_buffer(uint64_t *a, uint64_t *b, uint64_t *result)
 {
   uint64_t t[8U] = { 0U };
@@ -1992,7 +1997,13 @@ static uint64_t *const_to_lbuffer__uint64_t(const uint64_t *b)
 }
 
 static void
-point_add_mixed(uint64_t *p, const uint64_t *q, uint64_t *result, uint64_t *tempBuffer)
+point_add_mixed(
+  Lib_Buffer_buftype buftype,
+  uint64_t *p,
+  void *q,
+  uint64_t *result,
+  uint64_t *tempBuffer
+)
 {
   uint64_t *tempBuffer28 = tempBuffer;
   uint64_t *tempBuffer16 = tempBuffer;
@@ -2007,14 +2018,60 @@ point_add_mixed(uint64_t *p, const uint64_t *q, uint64_t *result, uint64_t *temp
   uint64_t *pX = p;
   uint64_t *pY = p + (uint32_t)4U;
   uint64_t *pZ = p + (uint32_t)8U;
-  const uint64_t *qX0 = q;
-  const uint64_t *qY0 = q + (uint32_t)4U;
+  void *qX0;
+  switch (buftype)
+  {
+    case Lib_Buffer_MUT:
+      {
+        qX0 = (void *)(uint64_t *)q;
+        break;
+      }
+    case Lib_Buffer_IMMUT:
+      {
+        qX0 = (void *)(uint64_t *)q;
+        break;
+      }
+    case Lib_Buffer_CONST:
+      {
+        qX0 = (void *)(const uint64_t *)q;
+        break;
+      }
+    default:
+      {
+        KRML_HOST_EPRINTF("KreMLin incomplete match at %s:%d\n", __FILE__, __LINE__);
+        KRML_HOST_EXIT(253U);
+      }
+  }
+  void *qY0;
+  switch (buftype)
+  {
+    case Lib_Buffer_MUT:
+      {
+        qY0 = (void *)((uint64_t *)q + (uint32_t)4U);
+        break;
+      }
+    case Lib_Buffer_IMMUT:
+      {
+        qY0 = (void *)((uint64_t *)q + (uint32_t)4U);
+        break;
+      }
+    case Lib_Buffer_CONST:
+      {
+        qY0 = (void *)((const uint64_t *)q + (uint32_t)4U);
+        break;
+      }
+    default:
+      {
+        KRML_HOST_EPRINTF("KreMLin incomplete match at %s:%d\n", __FILE__, __LINE__);
+        KRML_HOST_EXIT(253U);
+      }
+  }
   uint64_t *z2Square = tempBuffer16;
   uint64_t *z1Square = tempBuffer16 + (uint32_t)4U;
   uint64_t *z2Cube = tempBuffer16 + (uint32_t)8U;
   uint64_t *z1Cube = tempBuffer16 + (uint32_t)12U;
-  uint64_t *qX10 = const_to_lbuffer__uint64_t(qX0);
-  uint64_t *qY10 = const_to_lbuffer__uint64_t(qY0);
+  uint64_t *qX10 = const_to_lbuffer__uint64_t((const uint64_t *)qX0);
+  uint64_t *qY10 = const_to_lbuffer__uint64_t((const uint64_t *)qY0);
   z2Square[0U] = (uint64_t)0x000000300000000U;
   z2Square[1U] = (uint64_t)0x00000001FFFFFFFEU;
   z2Square[2U] = (uint64_t)0xFFFFFFFD00000002U;
@@ -2365,10 +2422,56 @@ point_add_mixed(uint64_t *p, const uint64_t *q, uint64_t *result, uint64_t *temp
   uint64_t *xOut1 = pointOut;
   uint64_t *yOut1 = pointOut + (uint32_t)4U;
   uint64_t *zOut1 = pointOut + (uint32_t)8U;
-  const uint64_t *qX = q;
-  const uint64_t *qY = q + (uint32_t)4U;
-  uint64_t *qX1 = const_to_lbuffer__uint64_t(qX);
-  uint64_t *qY1 = const_to_lbuffer__uint64_t(qY);
+  void *qX;
+  switch (buftype)
+  {
+    case Lib_Buffer_MUT:
+      {
+        qX = (void *)(uint64_t *)q;
+        break;
+      }
+    case Lib_Buffer_IMMUT:
+      {
+        qX = (void *)(uint64_t *)q;
+        break;
+      }
+    case Lib_Buffer_CONST:
+      {
+        qX = (void *)(const uint64_t *)q;
+        break;
+      }
+    default:
+      {
+        KRML_HOST_EPRINTF("KreMLin incomplete match at %s:%d\n", __FILE__, __LINE__);
+        KRML_HOST_EXIT(253U);
+      }
+  }
+  void *qY;
+  switch (buftype)
+  {
+    case Lib_Buffer_MUT:
+      {
+        qY = (void *)((uint64_t *)q + (uint32_t)4U);
+        break;
+      }
+    case Lib_Buffer_IMMUT:
+      {
+        qY = (void *)((uint64_t *)q + (uint32_t)4U);
+        break;
+      }
+    case Lib_Buffer_CONST:
+      {
+        qY = (void *)((const uint64_t *)q + (uint32_t)4U);
+        break;
+      }
+    default:
+      {
+        KRML_HOST_EPRINTF("KreMLin incomplete match at %s:%d\n", __FILE__, __LINE__);
+        KRML_HOST_EXIT(253U);
+      }
+  }
+  uint64_t *qX1 = const_to_lbuffer__uint64_t((const uint64_t *)qX);
+  uint64_t *qY1 = const_to_lbuffer__uint64_t((const uint64_t *)qY);
   uint64_t out_0 = xOut1[0U];
   uint64_t out_10 = xOut1[1U];
   uint64_t out_20 = xOut1[2U];
@@ -2417,9 +2520,55 @@ point_add_mixed(uint64_t *p, const uint64_t *q, uint64_t *result, uint64_t *temp
   zOut1[1U] = r_1;
   zOut1[2U] = r_2;
   zOut1[3U] = r_3;
-  const uint64_t *x = q;
-  const uint64_t *y = q + (uint32_t)4U;
-  uint64_t *uu____4 = global_to_comparable(x);
+  void *x;
+  switch (buftype)
+  {
+    case Lib_Buffer_MUT:
+      {
+        x = (void *)(uint64_t *)q;
+        break;
+      }
+    case Lib_Buffer_IMMUT:
+      {
+        x = (void *)(uint64_t *)q;
+        break;
+      }
+    case Lib_Buffer_CONST:
+      {
+        x = (void *)(const uint64_t *)q;
+        break;
+      }
+    default:
+      {
+        KRML_HOST_EPRINTF("KreMLin incomplete match at %s:%d\n", __FILE__, __LINE__);
+        KRML_HOST_EXIT(253U);
+      }
+  }
+  void *y;
+  switch (buftype)
+  {
+    case Lib_Buffer_MUT:
+      {
+        y = (void *)((uint64_t *)q + (uint32_t)4U);
+        break;
+      }
+    case Lib_Buffer_IMMUT:
+      {
+        y = (void *)((uint64_t *)q + (uint32_t)4U);
+        break;
+      }
+    case Lib_Buffer_CONST:
+      {
+        y = (void *)((const uint64_t *)q + (uint32_t)4U);
+        break;
+      }
+    default:
+      {
+        KRML_HOST_EPRINTF("KreMLin incomplete match at %s:%d\n", __FILE__, __LINE__);
+        KRML_HOST_EXIT(253U);
+      }
+  }
+  uint64_t *uu____4 = global_to_comparable((const uint64_t *)x);
   uint64_t a05 = uu____4[0U];
   uint64_t a15 = uu____4[1U];
   uint64_t a21 = uu____4[2U];
@@ -2431,7 +2580,7 @@ point_add_mixed(uint64_t *p, const uint64_t *q, uint64_t *result, uint64_t *temp
   uint64_t r013 = r012 & r110;
   uint64_t r231 = r211 & r310;
   uint64_t xZero = r013 & r231;
-  uint64_t *uu____5 = global_to_comparable(y);
+  uint64_t *uu____5 = global_to_comparable((const uint64_t *)y);
   uint64_t a0 = uu____5[0U];
   uint64_t a1 = uu____5[1U];
   uint64_t a2 = uu____5[2U];
@@ -2456,6 +2605,239 @@ point_add_mixed(uint64_t *p, const uint64_t *q, uint64_t *result, uint64_t *temp
   cmovznz4(p_x, x_x, result_x, mask0);
   cmovznz4(p_y, x_y, result_y, mask0);
   cmovznz4(p_z, x_z, result_z, mask0);
+}
+
+static const
+uint64_t
+points_cmb[128U] =
+  {
+    (uint64_t)0x0U, (uint64_t)0x0U, (uint64_t)0x0U, (uint64_t)0x0U, (uint64_t)0x0U, (uint64_t)0x0U,
+    (uint64_t)0x0U, (uint64_t)0x0U, (uint64_t)0x1fb38ab1388ad777U, (uint64_t)0x1dfee06615fa309dU,
+    (uint64_t)0xfcac986c3afea4a7U, (uint64_t)0xdf65c2da29fb821aU, (uint64_t)0xeff44e23f63f8f6dU,
+    (uint64_t)0xaa02cd3ed4b681a4U, (uint64_t)0xdd5fda3363818af8U, (uint64_t)0xfc53bc2629fbf0b3U,
+    (uint64_t)0x12631d721b91beeaU, (uint64_t)0x5f73f2d3a11a09f8U, (uint64_t)0xac41f54484d5fcd8U,
+    (uint64_t)0x86578e5c56025df4U, (uint64_t)0x577c956b15ed6b5aU, (uint64_t)0xb59c5f77982d848U,
+    (uint64_t)0xb7c5e2c190fcdcc2U, (uint64_t)0x7d64d13ef1c91ffdU, (uint64_t)0xd40c2d6273f9d9f1U,
+    (uint64_t)0x4dc6f628063ef17cU, (uint64_t)0x498e81df7ab17aa5U, (uint64_t)0xabb2a5026f17173cU,
+    (uint64_t)0x4a3d7527f6739ef3U, (uint64_t)0xd941003268184c91U, (uint64_t)0xd2d458b8d401508bU,
+    (uint64_t)0xb7437ab810ac5451U, (uint64_t)0x5256d9bdab491252U, (uint64_t)0x972d326eb1084c12U,
+    (uint64_t)0xc3e96455e2ec3bfaU, (uint64_t)0xb75c723b549a10ffU, (uint64_t)0x9d9185f9f8a18961U,
+    (uint64_t)0x2200a07b8589ba82U, (uint64_t)0x637b9d96fd4e9f5eU, (uint64_t)0xce75bfb2575e6cfaU,
+    (uint64_t)0x7dd4477db8b77c7dU, (uint64_t)0x80818a776e5503b0U, (uint64_t)0x6fc7d58fb59581dU,
+    (uint64_t)0xd899fb87efe43022U, (uint64_t)0x23b9912111694135U, (uint64_t)0x7e5de7bac33fa1c8U,
+    (uint64_t)0xb3b83722a70e7d43U, (uint64_t)0xf06cfecbfb9bb38fU, (uint64_t)0xaa39277dfa93656U,
+    (uint64_t)0x3dabb6cce67c5201U, (uint64_t)0x473ffb8bf1f94677U, (uint64_t)0xb9f0b93637453e56U,
+    (uint64_t)0x8fce12ec20958fb2U, (uint64_t)0xcc16d74ff7786061U, (uint64_t)0x3678438a8235d096U,
+    (uint64_t)0xe39ea044f06b43f6U, (uint64_t)0xbb40bdb5775c9950U, (uint64_t)0xd244a74cdc703cddU,
+    (uint64_t)0x83dc1b8a6105dd53U, (uint64_t)0x38d9d50d49ef0437U, (uint64_t)0x58be44eba6096472U,
+    (uint64_t)0x960afaec386fa5c5U, (uint64_t)0x1440032e000134b9U, (uint64_t)0x601e721454d6ba96U,
+    (uint64_t)0x79ec42228671b9b6U, (uint64_t)0xfdc00dc48df9e25cU, (uint64_t)0x44500833d71d2e77U,
+    (uint64_t)0x2bda4c3c0bc103d5U, (uint64_t)0x51528408aa925d53U, (uint64_t)0xefcb55b9c2f3a37dU,
+    (uint64_t)0x9f28f6bb9846c915U, (uint64_t)0xe1547ce1d8340e55U, (uint64_t)0x97e310c1995b3ed2U,
+    (uint64_t)0xed861937196256e6U, (uint64_t)0x1c6762abff2c65f2U, (uint64_t)0x268345e0978fceddU,
+    (uint64_t)0x35ca2e572b784881U, (uint64_t)0x28ac888da0acd1b7U, (uint64_t)0x305640dc06a41bafU,
+    (uint64_t)0x997c6fd2cb671bfbU, (uint64_t)0xf40d9eaf4a31e15aU, (uint64_t)0x8991dd7d54cfe03aU,
+    (uint64_t)0x4889a3463a8deb0cU, (uint64_t)0x4cbf48092cd0a1faU, (uint64_t)0xc6965c4fbe18fb8cU,
+    (uint64_t)0x1d499d0cb216fa84U, (uint64_t)0x8d5fe52c705dd3ebU, (uint64_t)0x812b268f84313b34U,
+    (uint64_t)0x313b58808261591aU, (uint64_t)0xc2c322508f53d933U, (uint64_t)0xa49ef3f95094ed1bU,
+    (uint64_t)0x13e326786e98c63U, (uint64_t)0x34be8167cd460429U, (uint64_t)0x698a328099a6b31U,
+    (uint64_t)0xb9be3ba51b0c922dU, (uint64_t)0xe59cca03f7674edU, (uint64_t)0x4fbf7e505d3aca7cU,
+    (uint64_t)0x2f4f8ba62020715U, (uint64_t)0x840502262ac1ec42U, (uint64_t)0xb8e0532775197de7U,
+    (uint64_t)0x9142a358cf4e9b4bU, (uint64_t)0xc86a3c567e5d8626U, (uint64_t)0xd4051282b4a7992aU,
+    (uint64_t)0xe7573c5999e3974eU, (uint64_t)0xd814a606da7bd76bU, (uint64_t)0x15604730f38cb788U,
+    (uint64_t)0xbd195f868fbdd6c4U, (uint64_t)0xdb96f5b00a51d3f7U, (uint64_t)0xe1385c8a9b507feaU,
+    (uint64_t)0x878e27813ee7310U, (uint64_t)0x6d7d8b12aea7e096U, (uint64_t)0x54978ad11e2f5ccaU,
+    (uint64_t)0x49fffd6c3c4d07d4U, (uint64_t)0x703638f71fab7a5dU, (uint64_t)0xbed6e367fcc73960U,
+    (uint64_t)0x215e161835a61d75U, (uint64_t)0xe52288a5e87a660bU, (uint64_t)0xf1d127ee3c802cb5U,
+    (uint64_t)0xccde3c6aafc46044U, (uint64_t)0xdc11c08ef14cff32U, (uint64_t)0x29216f9ceca46668U,
+    (uint64_t)0x22e584a3b2891c5eU, (uint64_t)0xe6deecd7810f6d87U, (uint64_t)0x6aff4b94a55659a3U,
+    (uint64_t)0x12b59bb6d2e9f876U, (uint64_t)0x27ed01943aa02eabU, (uint64_t)0x8d6d420841f57075U,
+    (uint64_t)0xe7b47285ef60a461U
+  };
+
+static uint64_t scalar_bit(uint8_t *s, uint32_t n)
+{
+  return (uint64_t)(s[n / (uint32_t)8U] >> n % (uint32_t)8U & (uint8_t)1U);
+}
+
+static void scalar_rwnaf(uint64_t *out, uint8_t *scalar)
+{
+  uint8_t in0 = scalar[0U];
+  uint64_t windowStartValue = (uint64_t)1U | ((uint64_t)in0 & (uint64_t)63U);
+  uint64_t window = windowStartValue;
+  uint64_t r = (uint64_t)0U;
+  uint64_t r1 = (uint64_t)0U;
+  for (uint32_t i = (uint32_t)0U; i < (uint32_t)51U; i++)
+  {
+    uint64_t wVar = window;
+    uint64_t w = wVar & (uint64_t)63U;
+    uint64_t d = (wVar & (uint64_t)63U) - (uint64_t)32U;
+    uint64_t c = Lib_IntTypes_Intrinsics_sub_borrow_u64((uint64_t)0U, w, (uint64_t)32U, &r);
+    uint64_t c1 = Lib_IntTypes_Intrinsics_sub_borrow_u64((uint64_t)0U, (uint64_t)0U, r, &r1);
+    uint64_t cAsFlag = (uint64_t)0xffffffffU + c;
+    uint64_t r3 = (r & cAsFlag) | (r1 & ~cAsFlag);
+    out[(uint32_t)2U * i] = r3;
+    out[(uint32_t)2U * i + (uint32_t)(krml_checked_int_t)1] = c;
+    uint64_t wStart = (wVar - d) >> (uint32_t)(uint64_t)5U;
+    uint64_t
+    w0 =
+      wStart
+      +
+        (scalar_bit(scalar,
+          ((uint32_t)1U + i) * (uint32_t)(uint64_t)5U + (uint32_t)1U)
+        << (uint32_t)1U);
+    uint64_t
+    w01 =
+      w0
+      +
+        (scalar_bit(scalar,
+          ((uint32_t)1U + i) * (uint32_t)(uint64_t)5U + (uint32_t)2U)
+        << (uint32_t)2U);
+    uint64_t
+    w02 =
+      w01
+      +
+        (scalar_bit(scalar,
+          ((uint32_t)1U + i) * (uint32_t)(uint64_t)5U + (uint32_t)3U)
+        << (uint32_t)3U);
+    uint64_t
+    w03 =
+      w02
+      +
+        (scalar_bit(scalar,
+          ((uint32_t)1U + i) * (uint32_t)(uint64_t)5U + (uint32_t)4U)
+        << (uint32_t)4U);
+    uint64_t
+    w04 =
+      w03
+      +
+        (scalar_bit(scalar,
+          ((uint32_t)1U + i) * (uint32_t)(uint64_t)5U + (uint32_t)5U)
+        << (uint32_t)5U);
+    window = w04;
+  }
+  out[102U] = window;
+}
+
+static void loopK(uint64_t d, uint64_t *point, uint32_t j)
+{
+  for (uint32_t i = (uint32_t)0U; i < (uint32_t)16U; i++)
+  {
+    uint64_t mask = FStar_UInt64_eq_mask(d, (uint64_t)j);
+    uint64_t *lut_cmb_x = const_to_lbuffer__uint64_t(points_cmb + j * (uint32_t)16U + i);
+    uint64_t
+    *lut_cmb_y = const_to_lbuffer__uint64_t(points_cmb + j * (uint32_t)16U + i + (uint32_t)4U);
+    uint64_t *uu____0 = point;
+    uint64_t out_00 = uu____0[0U];
+    uint64_t out_10 = uu____0[1U];
+    uint64_t out_20 = uu____0[2U];
+    uint64_t out_30 = uu____0[3U];
+    uint64_t x_00 = lut_cmb_x[0U];
+    uint64_t x_10 = lut_cmb_x[1U];
+    uint64_t x_20 = lut_cmb_x[2U];
+    uint64_t x_30 = lut_cmb_x[3U];
+    uint64_t r_00 = out_00 ^ (mask & (out_00 ^ x_00));
+    uint64_t r_10 = out_10 ^ (mask & (out_10 ^ x_10));
+    uint64_t r_20 = out_20 ^ (mask & (out_20 ^ x_20));
+    uint64_t r_30 = out_30 ^ (mask & (out_30 ^ x_30));
+    uu____0[0U] = r_00;
+    uu____0[1U] = r_10;
+    uu____0[2U] = r_20;
+    uu____0[3U] = r_30;
+    uint64_t *uu____1 = point + (uint32_t)4U;
+    uint64_t out_0 = uu____1[0U];
+    uint64_t out_1 = uu____1[1U];
+    uint64_t out_2 = uu____1[2U];
+    uint64_t out_3 = uu____1[3U];
+    uint64_t x_0 = lut_cmb_y[0U];
+    uint64_t x_1 = lut_cmb_y[1U];
+    uint64_t x_2 = lut_cmb_y[2U];
+    uint64_t x_3 = lut_cmb_y[3U];
+    uint64_t r_0 = out_0 ^ (mask & (out_0 ^ x_0));
+    uint64_t r_1 = out_1 ^ (mask & (out_1 ^ x_1));
+    uint64_t r_2 = out_2 ^ (mask & (out_2 ^ x_2));
+    uint64_t r_3 = out_3 ^ (mask & (out_3 ^ x_3));
+    uu____1[0U] = r_0;
+    uu____1[1U] = r_1;
+    uu____1[2U] = r_2;
+    uu____1[3U] = r_3;
+  }
+}
+
+static void conditional_substraction(uint64_t *result)
+{
+  
+}
+
+static void scalar_multiplication_cmb(uint64_t *result, void *scalar, uint64_t *tempBuffer)
+{
+  uint64_t rnaf2[104U] = { 0U };
+  uint64_t q[12U] = { 0U };
+  uint64_t lut[8U] = { 0U };
+  scalar_rwnaf(rnaf2, (uint8_t *)scalar);
+  uint32_t i0 = (uint32_t)1U;
+  for (uint32_t i = (uint32_t)0U; i < (uint32_t)16U; i++)
+  {
+    uint64_t d = rnaf2[(uint32_t)2U * (i * (uint32_t)2U + i0)];
+    uint64_t is_neg = rnaf2[(uint32_t)2U * (i * (uint32_t)2U + i0) + (uint32_t)1U];
+    uint64_t d1 = (d - (uint64_t)(uint32_t)1U) >> (uint32_t)1U;
+    uint64_t diff = FStar_UInt64_eq_mask(d1, (uint64_t)i);
+    loopK(diff, lut, i);
+    uint64_t *yLut = lut + (uint32_t)4U;
+    uint64_t *resultTemp = result;
+    p256_neg(yLut);
+    uint64_t out_0 = yLut[0U];
+    uint64_t out_1 = yLut[1U];
+    uint64_t out_2 = yLut[2U];
+    uint64_t out_3 = yLut[3U];
+    uint64_t x_0 = resultTemp[0U];
+    uint64_t x_1 = resultTemp[1U];
+    uint64_t x_2 = resultTemp[2U];
+    uint64_t x_3 = resultTemp[3U];
+    uint64_t r_0 = out_0 ^ (is_neg & (out_0 ^ x_0));
+    uint64_t r_1 = out_1 ^ (is_neg & (out_1 ^ x_1));
+    uint64_t r_2 = out_2 ^ (is_neg & (out_2 ^ x_2));
+    uint64_t r_3 = out_3 ^ (is_neg & (out_3 ^ x_3));
+    yLut[0U] = r_0;
+    yLut[1U] = r_1;
+    yLut[2U] = r_2;
+    yLut[3U] = r_3;
+    point_add_mixed(Lib_Buffer_MUT, q, (void *)lut, q, tempBuffer);
+  }
+  uint32_t i1 = (uint32_t)0U;
+  for (uint32_t i = (uint32_t)0U; i < (uint32_t)(uint64_t)5U; i++)
+  {
+    point_double(q, q, tempBuffer);
+  }
+  for (uint32_t i = (uint32_t)0U; i < (uint32_t)16U; i++)
+  {
+    uint64_t d = rnaf2[(uint32_t)2U * (i * (uint32_t)2U + i1)];
+    uint64_t is_neg = rnaf2[(uint32_t)2U * (i * (uint32_t)2U + i1) + (uint32_t)1U];
+    uint64_t d1 = (d - (uint64_t)(uint32_t)1U) >> (uint32_t)1U;
+    uint64_t diff = FStar_UInt64_eq_mask(d1, (uint64_t)i);
+    loopK(diff, lut, i);
+    uint64_t *yLut = lut + (uint32_t)4U;
+    uint64_t *resultTemp = result;
+    p256_neg(yLut);
+    uint64_t out_0 = yLut[0U];
+    uint64_t out_1 = yLut[1U];
+    uint64_t out_2 = yLut[2U];
+    uint64_t out_3 = yLut[3U];
+    uint64_t x_0 = resultTemp[0U];
+    uint64_t x_1 = resultTemp[1U];
+    uint64_t x_2 = resultTemp[2U];
+    uint64_t x_3 = resultTemp[3U];
+    uint64_t r_0 = out_0 ^ (is_neg & (out_0 ^ x_0));
+    uint64_t r_1 = out_1 ^ (is_neg & (out_1 ^ x_1));
+    uint64_t r_2 = out_2 ^ (is_neg & (out_2 ^ x_2));
+    uint64_t r_3 = out_3 ^ (is_neg & (out_3 ^ x_3));
+    yLut[0U] = r_0;
+    yLut[1U] = r_1;
+    yLut[2U] = r_2;
+    yLut[3U] = r_3;
+    point_add_mixed(Lib_Buffer_MUT, q, (void *)lut, q, tempBuffer);
+  }
+  conditional_substraction(q);
 }
 
 static inline uint64_t isPointAtInfinityPrivate(uint64_t *p)
@@ -3371,6 +3753,24 @@ scalarMultiplicationL(
         }
         break;
       }
+    case Spec_P256_Comb:
+      {
+        for (uint32_t i = (uint32_t)0U; i < (uint32_t)256U; i++)
+        {
+          uint32_t bit0 = (uint32_t)255U - i;
+          uint64_t
+          bit =
+            (uint64_t)(scalar[(uint32_t)31U
+            - bit0 / (uint32_t)8U]
+            >> bit0 % (uint32_t)8U
+            & (uint8_t)1U);
+          cswap(bit, q, result);
+          point_add(q, result, result, buff);
+          point_double(q, q, buff);
+          cswap(bit, q, result);
+        }
+        break;
+      }
     default:
       {
         KRML_HOST_EPRINTF("KreMLin incomplete match at %s:%d\n", __FILE__, __LINE__);
@@ -3457,6 +3857,24 @@ scalarMultiplicationC(
         break;
       }
     case Spec_P256_Radix4:
+      {
+        for (uint32_t i = (uint32_t)0U; i < (uint32_t)256U; i++)
+        {
+          uint32_t bit0 = (uint32_t)255U - i;
+          uint64_t
+          bit =
+            (uint64_t)(scalar[(uint32_t)31U
+            - bit0 / (uint32_t)8U]
+            >> bit0 % (uint32_t)8U
+            & (uint8_t)1U);
+          cswap(bit, q, result);
+          point_add(q, result, result, buff);
+          point_double(q, q, buff);
+          cswap(bit, q, result);
+        }
+        break;
+      }
+    case Spec_P256_Comb:
       {
         for (uint32_t i = (uint32_t)0U; i < (uint32_t)256U; i++)
         {
@@ -3869,8 +4287,29 @@ bool Hacl_P256_ecp256dh_i_radix4(uint8_t *result, uint8_t *scalar)
     point_double(resultBuffer, resultBuffer, buff);
     point_double(resultBuffer, resultBuffer, buff);
     point_double(resultBuffer, resultBuffer, buff);
-    point_add_mixed(resultBuffer, pointToAdd, resultBuffer, buff);
+    point_add_mixed(Lib_Buffer_CONST, resultBuffer, (void *)pointToAdd, resultBuffer, buff);
   }
+  norm(resultBuffer, resultBuffer, buff);
+  uint64_t flag = isPointAtInfinityPrivate(resultBuffer);
+  fromFormPoint(resultBuffer, result);
+  return flag == (uint64_t)0U;
+}
+
+/*
+ Input: result: uint8[64], 
+ scalar: uint8[32].
+  
+ Output: bool, where True stands for the correct key generation. 
+  
+ False means that an error has occurred (possibly that the result respresents point at infinity). 
+  
+*/
+bool Hacl_P256_ecp256dh_i_cmb(uint8_t *result, uint8_t *scalar)
+{
+  uint64_t tempBuffer[100U] = { 0U };
+  uint64_t resultBuffer[12U] = { 0U };
+  uint64_t *buff = tempBuffer + (uint32_t)12U;
+  scalar_multiplication_cmb(resultBuffer, (void *)scalar, buff);
   norm(resultBuffer, resultBuffer, buff);
   uint64_t flag = isPointAtInfinityPrivate(resultBuffer);
   fromFormPoint(resultBuffer, result);
@@ -3953,75 +4392,11 @@ bool Hacl_P256_ecp256dh_r_radix4(uint8_t *result, uint8_t *pubKey, uint8_t *scal
 
 void Hacl_P256_scalar_rwnaf(uint64_t *out, uint8_t *scalar)
 {
-  uint8_t in0 = scalar[0U];
-  uint64_t windowStartValue = (uint64_t)1U | ((uint64_t)in0 & (uint64_t)63U);
-  uint64_t window = windowStartValue;
-  uint64_t r = (uint64_t)0U;
-  uint64_t r1 = (uint64_t)0U;
-  for (uint32_t i = (uint32_t)0U; i < (uint32_t)51U; i++)
-  {
-    uint64_t wVar = window;
-    uint64_t w = wVar & (uint64_t)63U;
-    uint64_t d = (wVar & (uint64_t)63U) - (uint64_t)32U;
-    uint64_t c = Lib_IntTypes_Intrinsics_sub_borrow_u64((uint64_t)0U, w, (uint64_t)32U, &r);
-    uint64_t c1 = Lib_IntTypes_Intrinsics_sub_borrow_u64((uint64_t)0U, (uint64_t)0U, r, &r1);
-    uint64_t cAsFlag = (uint64_t)0xffffffffU + c;
-    uint64_t r3 = (r & cAsFlag) | (r1 & ~cAsFlag);
-    out[(uint32_t)2U * i] = r3;
-    out[(uint32_t)2U * i + (uint32_t)(krml_checked_int_t)1] = c;
-    uint64_t wStart = (wVar - d) >> (uint32_t)(uint64_t)5U;
-    uint64_t
-    w0 =
-      wStart
-      +
-        ((uint64_t)(scalar[(((uint32_t)1U + i) * (uint32_t)(uint64_t)5U + (uint32_t)1U)
-        / (uint32_t)8U]
-        >> (((uint32_t)1U + i) * (uint32_t)(uint64_t)5U + (uint32_t)1U) % (uint32_t)8U
-        & (uint8_t)1U)
-        << (uint32_t)1U);
-    uint64_t
-    w01 =
-      w0
-      +
-        ((uint64_t)(scalar[(((uint32_t)1U + i) * (uint32_t)(uint64_t)5U + (uint32_t)2U)
-        / (uint32_t)8U]
-        >> (((uint32_t)1U + i) * (uint32_t)(uint64_t)5U + (uint32_t)2U) % (uint32_t)8U
-        & (uint8_t)1U)
-        << (uint32_t)2U);
-    uint64_t
-    w02 =
-      w01
-      +
-        ((uint64_t)(scalar[(((uint32_t)1U + i) * (uint32_t)(uint64_t)5U + (uint32_t)3U)
-        / (uint32_t)8U]
-        >> (((uint32_t)1U + i) * (uint32_t)(uint64_t)5U + (uint32_t)3U) % (uint32_t)8U
-        & (uint8_t)1U)
-        << (uint32_t)3U);
-    uint64_t
-    w03 =
-      w02
-      +
-        ((uint64_t)(scalar[(((uint32_t)1U + i) * (uint32_t)(uint64_t)5U + (uint32_t)4U)
-        / (uint32_t)8U]
-        >> (((uint32_t)1U + i) * (uint32_t)(uint64_t)5U + (uint32_t)4U) % (uint32_t)8U
-        & (uint8_t)1U)
-        << (uint32_t)4U);
-    uint64_t
-    w04 =
-      w03
-      +
-        ((uint64_t)(scalar[(((uint32_t)1U + i) * (uint32_t)(uint64_t)5U + (uint32_t)5U)
-        / (uint32_t)8U]
-        >> (((uint32_t)1U + i) * (uint32_t)(uint64_t)5U + (uint32_t)5U) % (uint32_t)8U
-        & (uint8_t)1U)
-        << (uint32_t)5U);
-    window = w04;
-  }
-  out[102U] = window;
+  scalar_rwnaf(out, scalar);
 }
 
 uint64_t Hacl_P256_scalar_bit(uint8_t *b, uint32_t c)
 {
-  return (uint64_t)(b[c / (uint32_t)8U] >> c % (uint32_t)8U & (uint8_t)1U);
+  return scalar_bit(b, c);
 }
 
