code/ecdsap256/dist/test.c
@@ -213,7 +213,7 @@ int main()
 		}
 
 
-		// return -1;
+		return -1;
 
 	printf("\n");
 
