code/ecdsap256/Hacl.Impl.ScalarMultiplication.WNAF.fst
@@ -16,11 +16,80 @@ open Lib.IntTypes.Intrinsics
 open Hacl.Impl.P256.Q.PrimitivesMasking
 
 
+open Spec.P256.Definitions
+open Hacl.Impl.P256.LowLevel.PrimeSpecific
+open Hacl.Impl.P256.PointDouble
+open Hacl.Impl.P256.MixedPointAdd
+
+(* let´s pretend that it´s 432 *)
+
+inline_for_extraction noextract
+let cmb_list: x:list uint64{List.Tot.length x == 432} =
+  let open FStar.Mul in 
+  [@inline_let]
+  let x = [ 
+    u64 0x0; u64 0x0; u64 0x0; u64 0x0; 
+    u64 0x0; u64 0x0; u64 0x0; u64 0x0; 
+
+    u64 0x1fb38ab1388ad777; u64 0x1dfee06615fa309d; u64 0xfcac986c3afea4a7; u64 0xdf65c2da29fb821a; 
+    u64 0xeff44e23f63f8f6d; u64 0xaa02cd3ed4b681a4; u64 0xdd5fda3363818af8; u64 0xfc53bc2629fbf0b3; 
+
+    u64 0x12631d721b91beea; u64 0x5f73f2d3a11a09f8; u64 0xac41f54484d5fcd8; u64 0x86578e5c56025df4; 
+    u64 0x577c956b15ed6b5a; u64 0xb59c5f77982d848; u64 0xb7c5e2c190fcdcc2; u64 0x7d64d13ef1c91ffd; 
+
+    u64 0xd40c2d6273f9d9f1; u64 0x4dc6f628063ef17c; u64 0x498e81df7ab17aa5; u64 0xabb2a5026f17173c; 
+    u64 0x4a3d7527f6739ef3; u64 0xd941003268184c91; u64 0xd2d458b8d401508b; u64 0xb7437ab810ac5451; 
+
+    u64 0x5256d9bdab491252; u64 0x972d326eb1084c12; u64 0xc3e96455e2ec3bfa; u64 0xb75c723b549a10ff; 
+    u64 0x9d9185f9f8a18961; u64 0x2200a07b8589ba82; u64 0x637b9d96fd4e9f5e; u64 0xce75bfb2575e6cfa; 
+
+    u64 0x7dd4477db8b77c7d; u64 0x80818a776e5503b0; u64 0x6fc7d58fb59581d; u64 0xd899fb87efe43022; 
+    u64 0x23b9912111694135; u64 0x7e5de7bac33fa1c8; u64 0xb3b83722a70e7d43; u64 0xf06cfecbfb9bb38f; 
+
+    u64 0xaa39277dfa93656; u64 0x3dabb6cce67c5201; u64 0x473ffb8bf1f94677; u64 0xb9f0b93637453e56; 
+    u64 0x8fce12ec20958fb2; u64 0xcc16d74ff7786061; u64 0x3678438a8235d096; u64 0xe39ea044f06b43f6; 
+
+    u64 0xbb40bdb5775c9950; u64 0xd244a74cdc703cdd; u64 0x83dc1b8a6105dd53; u64 0x38d9d50d49ef0437; 
+    u64 0x58be44eba6096472; u64 0x960afaec386fa5c5; u64 0x1440032e000134b9; u64 0x601e721454d6ba96; 
+
+    u64 0x79ec42228671b9b6; u64 0xfdc00dc48df9e25c; u64 0x44500833d71d2e77; u64 0x2bda4c3c0bc103d5; 
+    u64 0x51528408aa925d53; u64 0xefcb55b9c2f3a37d; u64 0x9f28f6bb9846c915; u64 0xe1547ce1d8340e55; 
+
+    u64 0x97e310c1995b3ed2; u64 0xed861937196256e6; u64 0x1c6762abff2c65f2; u64 0x268345e0978fcedd; 
+    u64 0x35ca2e572b784881; u64 0x28ac888da0acd1b7; u64 0x305640dc06a41baf; u64 0x997c6fd2cb671bfb; 
+
+    u64 0xf40d9eaf4a31e15a; u64 0x8991dd7d54cfe03a; u64 0x4889a3463a8deb0c; u64 0x4cbf48092cd0a1fa; 
+    u64 0xc6965c4fbe18fb8c; u64 0x1d499d0cb216fa84; u64 0x8d5fe52c705dd3eb; u64 0x812b268f84313b34; 
+
+    u64 0x313b58808261591a; u64 0xc2c322508f53d933; u64 0xa49ef3f95094ed1b; u64 0x13e326786e98c63; 
+    u64 0x34be8167cd460429; u64 0x698a328099a6b31; u64 0xb9be3ba51b0c922d; u64 0xe59cca03f7674ed; 
+    
+    u64 0x4fbf7e505d3aca7c; u64 0x2f4f8ba62020715; u64 0x840502262ac1ec42; u64 0xb8e0532775197de7; 
+    u64 0x9142a358cf4e9b4b; u64 0xc86a3c567e5d8626; u64 0xd4051282b4a7992a; u64 0xe7573c5999e3974e;
+    
+    u64 0xd814a606da7bd76b; u64 0x15604730f38cb788; u64 0xbd195f868fbdd6c4; u64 0xdb96f5b00a51d3f7; 
+    u64 0xe1385c8a9b507fea; u64 0x878e27813ee7310; u64 0x6d7d8b12aea7e096; u64 0x54978ad11e2f5cca; 
+    
+    u64 0x49fffd6c3c4d07d4; u64 0x703638f71fab7a5d; u64 0xbed6e367fcc73960; u64 0x215e161835a61d75; 
+    u64 0xe52288a5e87a660b; u64 0xf1d127ee3c802cb5; u64 0xccde3c6aafc46044; u64 0xdc11c08ef14cff32; 
+
+    u64 0x29216f9ceca46668; u64 0x22e584a3b2891c5e; u64 0xe6deecd7810f6d87; u64 0x6aff4b94a55659a3; 
+   u64 0x12b59bb6d2e9f876; u64 0x27ed01943aa02eab; u64 0x8d6d420841f57075; u64 0xe7b47285ef60a461;  
+  ] in x
+
+
+
+inline_for_extraction
+let points_cmb : x: glbuffer uint64 432ul {witnessed #uint64 #(size 432) x (Lib.Sequence.of_list cmb_list) /\ recallable x} =
+    createL_global cmb_list
+
+
+
+
 (* Originally lives in P256.Core *)
 (* this piece of code is taken from Hacl.Curve25519 *)
 (* changed Endian for Scalar Bit access *)
 
-inline_for_extraction
 val scalar_bit:
     s:lbuffer_t MUT uint8 (size 32)
   -> n:size_t{v n < 256}
@@ -44,7 +113,7 @@ let dradix = (u64 32)
 inline_for_extraction noextract
 let radix = (u64 5)
 
-inline_for_extraction noextract
+(* I work *)
 val scalar_rwnaf : out: lbuffer uint64 (size 104) -> scalar: lbuffer uint8 (size 32) -> 
   Stack unit 
     (requires fun h -> live h out /\ live h scalar)
@@ -101,7 +170,115 @@ let scalar_rwnaf out scalar =
     upd out (size 102) (index window (size 0));
 
 pop_frame()
+
+
+
+inline_for_extraction
+type pointAffine = lbuffer uint64 (size 8)
+
+
+val loopK: result: pointAffine -> d: uint64 -> point: pointAffine -> j: size_t ->  Stack unit 
+  (requires fun h -> True)
+  (ensures fun h0 _ h1 -> True)
+
+let loopK result d point j = 
+  let invK h (k: nat) = True in 
+  Lib.Loops.for 0ul 16ul invK
+    (fun k -> 
+      let mask = eq_mask d (to_u64 j) in 
+      let lut_cmb_x = const_to_lbuffer (sub points_cmb (j *! size 16 +! k) (size 4)) in 
+      let lut_cmb_y = const_to_lbuffer (sub points_cmb (j *! size 16 +! k +! (size 4)) (size 4)) in 
+
+      
+
+      copy_conditional (sub point (size 0) (size 4)) lut_cmb_x mask;
+      copy_conditional (sub point (size 4) (size 4)) lut_cmb_y mask
+    )
+
   
 
 
+val conditional_substraction: result: point -> p: point -> 
+  Stack unit 
+    (requires fun h -> True)
+    (ensures fun h0 _ h1 -> True)
 
+
+let conditional_substraction result p = ()
+
+
+
+
+val scalar_multiplication_cmb:  #buf_type: buftype -> result: point -> 
+  scalar: lbuffer_t buf_type uint8 (size 32) -> 
+  tempBuffer:  lbuffer uint64 (size 88)  -> 
+  Stack unit
+  (requires fun h -> True )
+  (ensures fun h0 _ h1 -> modifies (loc result |+| loc tempBuffer) h0 h1)
+
+
+let scalar_multiplication_cmb #buf_type result scalar tempBuffer = 
+  push_frame();
+    let rnaf2 = create (size 104) (u64 0) in 
+
+    (* point_at_infinity *)
+    let q = create (size 12) (u64 0) in 
+    let lut:pointAffine = create (size 8) (u64 0) in 
+
+    scalar_rwnaf rnaf2 scalar;
+
+    let i = size 1 in 
+
+    let invJ h1 (j:nat) = True in  
+
+    Lib.Loops.for 0ul 16ul invJ
+      (fun j ->
+	let d = index rnaf2 (size 2 *! (j *! (size 2) +! i)) in 
+	let is_neg = index rnaf2 (size 2 *! (j *! (size 2) +! i) +! (size 1)) in 
+	let d = shift_right (d -! size 1) (size 1) in 
+
+	let diff = eq_mask d (to_u64 j) in 
+
+	loopK lut diff lut j;
+
+	let yLut = sub lut (size 4) (size 4) in 
+	let resultTemp = sub result (size 0) (size 4) in 
+	p256_neg yLut resultTemp;
+
+	
+	copy_conditional yLut resultTemp is_neg;
+	point_add_mixed q lut q tempBuffer);
+     
+
+  let i = size 0 in 
+
+  let invPointDouble h (j: nat) = True in 
+  Lib.Loops.for 0ul radix invPointDouble 
+    (fun j -> 
+      point_double q q tempBuffer);
+
+
+  
+    Lib.Loops.for 0ul 16ul invJ
+      (fun j ->
+	let d = index rnaf2 (size 2 *! (j *! (size 2) +! i)) in 
+	let is_neg = index rnaf2 (size 2 *! (j *! (size 2) +! i) +! (size 1)) in 
+	let d = shift_right (d -! size 1) (size 1) in 
+
+	let diff = eq_mask d (to_u64 j) in 
+
+	loopK lut diff lut j;
+
+	let yLut = sub lut (size 4) (size 4) in 
+	let resultTemp = sub result (size 0) (size 4) in 
+	p256_neg yLut resultTemp;
+
+	
+	copy_conditional yLut resultTemp is_neg;
+	point_add_mixed q lut q tempBuffer);
+
+
+  conditional_substraction q q;
+  
+
+  pop_frame()
